

2.2

$$\begin{aligned}
 (x + y) \cdot (x + \overline{y}) &= xx + xy + x\overline{y} + y\overline{y} \\
 &= x + xy + x\overline{y} + 0 \\
 &= x(1 + y + \overline{y}) \\
 &= x \cdot 1 \\
 &= x
 \end{aligned}$$

2.10

$$\begin{aligned}
 f &= \overline{x}_1\overline{x}_2x_3 + \overline{x}_1x_2\overline{x}_3 + \overline{x}_1x_2x_3 + x_1\overline{x}_2\overline{x}_3 + x_1\overline{x}_2x_3 + x_1x_2\overline{x}_3 + x_1x_2x_3 \\
 &= x_1(\overline{x}_2\overline{x}_3 + \overline{x}_2x_3 + x_2\overline{x}_3 + x_2x_3) + x_2(\overline{x}_1\overline{x}_3 + \overline{x}_1x_3 + x_1\overline{x}_3 + x_1x_3) \\
 &\quad + x_3(\overline{x}_1\overline{x}_2 + \overline{x}_1x_2 + x_1\overline{x}_2 + x_1x_2) \\
 &= x_1(\overline{x}_2(\overline{x}_3 + x_3) + x_2(\overline{x}_3 + x_3)) + x_2(\overline{x}_1(\overline{x}_3 + x_3) + x_1(\overline{x}_3 + x_3)) \\
 &\quad + x_3(\overline{x}_1(\overline{x}_2 + x_2) + x_1(\overline{x}_2 + x_2)) \\
 &= x_1(\overline{x}_2 \cdot 1 + x_2 \cdot 1) + x_2(\overline{x}_1 \cdot 1 + x_1 \cdot 1) + x_3(\overline{x}_1 \cdot 1 + x_1 \cdot 1) \\
 &= x_1(\overline{x}_2 + x_2) + x_2(\overline{x}_1 + x_1) + x_3(\overline{x}_1 + x_1) \\
 &= x_1 \cdot 1 + x_2 \cdot 1 + x_3 \cdot 1 \\
 &= x_1 + x_2 + x_3
 \end{aligned}$$

2.13

$$\begin{aligned}
 f &= x_1\overline{x}_2\overline{x}_3 + x_1x_2x_4 + x_1\overline{x}_2x_3\overline{x}_4 \\
 &= x_1\overline{x}_2\overline{x}_3(\overline{x}_4 + x_4) + x_1x_2x_4 + x_1\overline{x}_2x_3\overline{x}_4 \\
 &= x_1\overline{x}_2\overline{x}_3\overline{x}_4 + x_1\overline{x}_2\overline{x}_3x_4 + x_1x_2x_4 + x_1\overline{x}_2x_3\overline{x}_4 \\
 &= x_1\overline{x}_2\overline{x}_3 + x_1\overline{x}_2(\overline{x}_3 + x_3)\overline{x}_4 + x_1x_2x_4 \\
 &= x_1\overline{x}_2\overline{x}_3 + x_1\overline{x}_2\overline{x}_4 + x_1x_2x_4
 \end{aligned}$$

2.24

$$\begin{aligned}
 f &= x_1\overline{x}_3\overline{x}_4 + x_2\overline{x}_3x_4 + x_1\overline{x}_2\overline{x}_3 \\
 &= x_1\overline{x}_3\overline{x}_4 + x_2\overline{x}_3x_4 + x_1x_2\overline{x}_3 + x_1\overline{x}_2\overline{x}_3 \\
 &= x_1\overline{x}_3\overline{x}_4 + x_2\overline{x}_3x_4 + x_1\overline{x}_3 \\
 &= x_2\overline{x}_3x_4 + x_1\overline{x}_3
 \end{aligned}$$

2.21

$$\begin{aligned}
 f &= \bar{x}_1 \bar{x}_2 x_3 + \bar{x}_1 x_2 x_3 + x_1 \bar{x}_2 \bar{x}_3 + x_1 x_2 \bar{x}_3 + x_1 x_2 x_3 \\
 &= \bar{x}_1 (\bar{x}_2 + x_2) x_3 + x_1 (\bar{x}_2 + x_2) \bar{x}_3 + (\bar{x}_1 + x_1) x_2 x_3 \\
 &= \bar{x}_1 x_3 + x_1 \bar{x}_3 + x_2 x_3
 \end{aligned}$$

$$f = \bar{x}_1 x_3 + x_1 \bar{x}_3 + x_1 x_2$$

3.2

- (a) 478
- (b) -280
- (c) -1

3.3

- (a) 478
- (b) -281
- (c) -2

3.8 (给出一种证明方法提示，详细步骤请自行补充)

证明

$$\begin{aligned}
 & \boxed{2^n} \cdot \begin{matrix} 0 & 0 & \dots & 0 & 0 & \dots & 0 & 0 \\ B_{n-1} & B_{n-2} & \dots & B_k & B_{k-1} & \dots & B_1 & B_0 \end{matrix} \\
 & \begin{matrix} 1 & 1 & 1 & \dots & 1 \\ 0 & 0 & 0 & \dots & 0 \end{matrix} \\
 & a = \begin{matrix} 1 & 1 & 1 & \dots & 1 \\ 0 & 0 & 0 & \dots & 0 \end{matrix} \\
 & b = \begin{matrix} 0 & 0 & 0 & \dots & 0 \\ 0 & 0 & 0 & \dots & 0 \end{matrix} \\
 & C = \{B_{n-1}, \dots, B_k\} \quad a+b-C \rightarrow \begin{cases} m_k = 1 \\ m_i = \bar{B}_i \quad k \leq i < n \end{cases}
 \end{aligned}$$

3.10

Since $s_k = x_k \oplus y_k \oplus c_k$, it follows that

$$\begin{aligned}x_k \oplus y_k \oplus s_k &= (x_k \oplus y_k) \oplus (x_k \oplus y_k \oplus c_k) \\&= (x_k \oplus y_k) \oplus (x_k \oplus y_k) \oplus c_k \\&= 0 \oplus c_k \\&= c_k\end{aligned}$$